Yet more metatheory for trans_alt

semantics/proofs/payload_altPropsScript.sml
@@ -29,8 +29,8 @@ Theorem ALOOKUP_ZIP_SELF:
 Proof
   Induct_on ‘l’ >>
   rw[] >> fs[]
-QED        
-        
+QED
+
 Theorem reduction_alt_IMP:
   ∀conf n1 n2.
     reduction_alt conf n1 n2 ⇒
@@ -98,8 +98,30 @@ Theorem RC_REFL:
   RC R x x
 Proof
   rw[RC_DEF]
-QED        
-        
+QED
+
+Theorem instacall_endpoint_dsubst:
+  ∀e1 dn e2.
+  instacall_endpoint e1 ∧ instacall_endpoint e2 ⇒
+  instacall_endpoint(dsubst e1 dn e2)
+Proof
+  rpt strip_tac >> Induct_on ‘e1’ >> rw[dsubst_def,instacall_endpoint_def]
+QED
+
+Theorem instacall_network_trans_pres:
+  ∀conf n1 α n2.
+    trans conf n1 α n2 ∧ instacall_network n1 ⇒ instacall_network n2
+Proof
+  simp[GSYM AND_IMP_INTRO] >>
+  ho_match_mp_tac trans_ind >> rpt strip_tac >>
+  fs[instacall_network_def,instacall_endpoint_def,instacall_closure_def,instacall_endpoint_dsubst] >>
+  CONV_TAC(DEPTH_CONV ETA_CONV) >> simp[] >>
+  imp_res_tac ALOOKUP_MEM >>
+  fs[EVERY_MEM,MEM_MAP,PULL_EXISTS] >>
+  res_tac >>
+  fs[instacall_closure_def,EVERY_MEM,MEM_MAP,PULL_EXISTS]
+QED
+
 Theorem reduction_IMP_reduction_alt:
   ∀conf n1 n2.
     reduction conf n1 n2 ∧
@@ -140,6 +162,1044 @@ Proof
   goal_assum(resolve_then (Pos last) mp_tac RC_REFL) >>
   simp[reduction_alt_def,Once trans_alt_cases] >>
   metis_tac[]
+QED
+
+Theorem instacall_network_trans_alt_pres:
+  ∀conf n1 α n2.
+    trans_alt conf n1 α n2 ∧ instacall_network n1 ⇒ instacall_network n2
+Proof
+  rpt strip_tac >>
+  Cases_on ‘α = LTau’ >-
+    (rveq >> fs[GSYM reduction_alt_def] >>
+     drule reduction_alt_IMP >>
+     pop_assum mp_tac >> simp[AND_IMP_INTRO] >>
+     match_mp_tac RTC_lifts_invariants >>
+     metis_tac[reduction_def,instacall_network_trans_pres]) >>
+  metis_tac[instacall_network_trans_pres,trans_alt_nontau_eq]
+QED
+
+Theorem trans_alt_send_receive_distinct:
+  trans_alt conf p1 (LSend s1 d1 r1) p2
+  /\ trans_alt conf p1 (LReceive s2 d2 r2) p3
+  /\ conf.payload_size > 0 (* not strictly needed *)
+  ==> p2 <> p3
+Proof
+  metis_tac[trans_send_receive_distinct,trans_alt_nontau_eq,label_distinct]
+QED
+
+Theorem trans_alt_different_sender:
+  trans_alt conf p1 (LSend s1 d1 r1) p2
+  /\ trans_alt conf p1 (LSend s2 d2 r2) p3
+  /\ conf.payload_size > 0
+  /\ s1 <> s2
+  ==> p2 <> p3
+Proof
+  metis_tac[trans_different_sender,trans_alt_nontau_eq,label_distinct]
+QED
+
+Theorem trans_alt_same_sender_determ:
+  trans_alt conf p1 (LSend q2 d1 q1) p2
+  /\ trans_alt conf p1 (LSend q2 d2 q3) p3
+  /\ ALL_DISTINCT(MAP FST(endpoints p1))
+  ==> q1 = q3 /\ d1 = d2 /\ p2 = p3
+Proof
+  metis_tac[trans_same_sender_determ,trans_alt_nontau_eq,label_distinct]
+QED
+
+Theorem sender_is_endpoint_alt:
+  ∀p1 p2 q1 d q2 conf.
+    trans_alt conf p1 (LSend q1 d q2) p2 ==> MEM q1 (MAP FST (endpoints p1))
+Proof
+  metis_tac[sender_is_endpoint,trans_alt_nontau_eq,label_distinct]
+QED
+
+Theorem receiver_is_endpoint_alt:
+  ∀p1 p2 q1 d q2 conf.
+    trans_alt conf p1 (LReceive q1 d q2) p2 ==> MEM q2 (MAP FST (endpoints p1))
+Proof
+  metis_tac[receiver_is_endpoint,trans_alt_nontau_eq,label_distinct]
+QED
+
+Theorem payload_local_confluence_send_alt:
+  ∀conf p1 alpha p2 p3 s d r.
+  trans_alt conf p1 alpha p2 /\ trans_alt conf p1 (LSend s d r) p3 /\ p2 <> p3 /\
+  ALL_DISTINCT (MAP FST (endpoints p1)) /\
+  ~MEM r (MAP FST (endpoints p1)) /\
+  conf.payload_size > 0
+  ==>
+  ?p4 p5. trans_alt conf p2 (LSend s d r) p4 /\
+        trans_alt conf p3 alpha p4
+Proof
+  simp[GSYM AND_IMP_INTRO, GSYM PULL_FORALL]
+  >> ho_match_mp_tac trans_alt_strongind
+  >> rpt strip_tac >> fs[] >> rveq
+  >- (* Send-last-payload *)
+     (qhdtm_x_assum `trans_alt` (assume_tac o SIMP_RULE std_ss [Once trans_alt_cases]) >>
+      fs[] >> rveq >> fs[] >> rveq >> fs[])
+  >- (* Send-intermediate-payload *)
+     (qhdtm_x_assum `trans_alt` (assume_tac o SIMP_RULE std_ss [Once trans_alt_cases]) >>
+      fs[] >> rveq >> fs[] >> rveq >> fs[])
+  >- (* Enqueue *)
+      (qhdtm_x_assum `trans_alt` (assume_tac o SIMP_RULE std_ss [Once trans_alt_cases]) >>
+       fs[] >> rveq >> fs[] >> rveq >> fs[]
+       >- (qmatch_goalsub_abbrev_tac `NEndpoint _ s1` >>
+           rename1 `FLOOKUP s.bindings v = SOME data` >>
+           `FLOOKUP s1.bindings v = SOME data` by simp[Abbr`s1`] >>
+           drule trans_alt_send_last_payload >> simp[] >>
+           disch_then drule >> disch_then dxrule >>
+           rename1 `Send _ _ _ e1` >>
+           disch_then(qspec_then `e1` assume_tac) >>
+           asm_exists_tac >> simp[] >>
+           drule trans_alt_enqueue >>
+           metis_tac[])
+       >- (qmatch_goalsub_abbrev_tac `NEndpoint _ s1` >>
+           rename1 `FLOOKUP s.bindings v = SOME data` >>
+           `FLOOKUP s1.bindings v = SOME data` by simp[Abbr`s1`] >>
+           drule trans_alt_send_last_payload >> simp[] >>
+           disch_then drule >> disch_then dxrule >>
+           rename1 `Send _ _ _ e1` >>
+           disch_then(qspec_then `e1` assume_tac) >>
+           asm_exists_tac >> simp[] >>
+           drule trans_alt_enqueue >>
+           metis_tac[])
+       >- (qmatch_goalsub_abbrev_tac `NEndpoint _ s1` >>
+           rename1 `FLOOKUP s.bindings v = SOME data` >>
+           `FLOOKUP s1.bindings v = SOME data` by simp[Abbr`s1`] >>
+           drule trans_alt_send_intermediate_payload >> simp[] >>
+           disch_then drule >> disch_then dxrule >>
+           rename1 `Send _ _ _ e1` >>
+           disch_then(qspec_then `e1` assume_tac) >>
+           asm_exists_tac >> simp[] >>
+           drule trans_alt_enqueue >>
+           metis_tac[]))
+  >- (* Com-L *)
+     (qhdtm_x_assum `trans_alt` (assume_tac o SIMP_RULE std_ss [Once trans_alt_cases]) >>
+      fs[] >> rveq >> fs[] >> rveq >> fs[]
+      >- (fs[endpoints_def,ALL_DISTINCT_APPEND] >>
+          first_x_assum(drule_all_then strip_assume_tac) >>
+          metis_tac[trans_alt_com_l,trans_alt_par_l])
+      >- (fs[endpoints_def,ALL_DISTINCT_APPEND] >>
+          first_x_assum drule >>
+          imp_res_tac sender_is_endpoint_alt >>
+          imp_res_tac receiver_is_endpoint_alt >>
+          Cases_on `s = p1''` (* TODO: generated names *)
+          >- metis_tac[trans_alt_same_sender_determ] >>
+          drule_then assume_tac (GEN_ALL trans_alt_different_sender) >>
+          qpat_x_assum `trans_alt _ _ (LSend _ _ _) _` mp_tac >>
+          pop_assum drule >> impl_tac >- simp[] >>
+          ntac 2 strip_tac >> impl_tac >- simp[] >>
+          strip_tac >> metis_tac[trans_alt_par_l,trans_alt_com_l])
+      >- (fs[endpoints_def,ALL_DISTINCT_APPEND] >>
+          first_x_assum drule >>
+          imp_res_tac sender_is_endpoint_alt >>
+          imp_res_tac receiver_is_endpoint_alt >>
+          impl_tac >- metis_tac[trans_alt_send_receive_distinct] >>
+          strip_tac >> metis_tac[trans_alt_par_r,trans_alt_com_l])
+      >- (fs[endpoints_def,ALL_DISTINCT_APPEND] >>
+          first_x_assum drule >>
+          imp_res_tac sender_is_endpoint_alt >>
+          imp_res_tac receiver_is_endpoint_alt >>
+          impl_tac >- metis_tac[trans_alt_send_receive_distinct] >>
+          strip_tac >> metis_tac[trans_alt_par_r,trans_alt_com_l]))
+  >- (* Com-R *)
+     (qhdtm_x_assum `trans_alt` (assume_tac o SIMP_RULE std_ss [Once trans_alt_cases]) >>
+      fs[] >> rveq >> fs[] >> rveq >> fs[]
+      >- (fs[endpoints_def,ALL_DISTINCT_APPEND] >>
+          first_x_assum(drule_all_then strip_assume_tac) >>
+          metis_tac[trans_alt_com_r,trans_alt_par_l])
+      >- (fs[endpoints_def,ALL_DISTINCT_APPEND] >>
+          last_x_assum drule >>
+          imp_res_tac sender_is_endpoint_alt >>
+          imp_res_tac receiver_is_endpoint_alt >>
+          impl_tac >- metis_tac[trans_alt_send_receive_distinct] >>
+          strip_tac >> metis_tac[trans_alt_par_l,trans_alt_com_r])
+      >- (fs[endpoints_def,ALL_DISTINCT_APPEND] >>
+          last_x_assum drule >>
+          imp_res_tac sender_is_endpoint_alt >>
+          imp_res_tac receiver_is_endpoint_alt >>
+          Cases_on `s = p1''` (* TODO: generated names *)
+          >- metis_tac[trans_alt_same_sender_determ] >>
+          drule_then assume_tac (GEN_ALL trans_alt_different_sender) >>
+          qpat_x_assum `trans_alt _ _ (LSend _ _ _) _` mp_tac >>
+          pop_assum drule >> impl_tac >- simp[] >>
+          ntac 2 strip_tac >> impl_tac >- simp[] >>
+          strip_tac >> metis_tac[trans_alt_par_r,trans_alt_com_r])
+      >- (fs[endpoints_def,ALL_DISTINCT_APPEND] >>
+          last_x_assum drule >>
+          imp_res_tac sender_is_endpoint_alt >>
+          imp_res_tac receiver_is_endpoint_alt >>
+          impl_tac >- metis_tac[trans_alt_send_receive_distinct] >>
+          strip_tac >> metis_tac[trans_alt_par_r,trans_alt_com_r]))
+  >- (* Dequeue-last-payload *)
+     (qhdtm_x_assum `trans_alt` (assume_tac o SIMP_RULE std_ss [Once trans_alt_cases]) >>
+      fs[] >> rveq >> fs[] >> rveq >> fs[])
+  >- (* Dequeue-intermediate-payload *)
+     (qhdtm_x_assum `trans_alt` (assume_tac o SIMP_RULE std_ss [Once trans_alt_cases]) >>
+      fs[] >> rveq >> fs[] >> rveq >> fs[])
+  >- (* If-L *)
+     (qhdtm_x_assum `trans_alt` (assume_tac o SIMP_RULE std_ss [Once trans_alt_cases]) >>
+      fs[] >> rveq >> fs[] >> rveq >> fs[])
+  >- (* If-R *)
+     (qhdtm_x_assum `trans_alt` (assume_tac o SIMP_RULE std_ss [Once trans_alt_cases]) >>
+      fs[] >> rveq >> fs[] >> rveq >> fs[])
+  >- (* Let *)
+     (qhdtm_x_assum `trans_alt` (assume_tac o SIMP_RULE std_ss [Once trans_alt_cases]) >>
+      fs[] >> rveq >> fs[] >> rveq >> fs[])
+  >- (* Par-L *)
+     (qhdtm_x_assum `trans_alt` (assume_tac o SIMP_RULE std_ss [Once trans_alt_cases]) >>
+      fs[] >> rveq >> fs[] >> rveq >> fs[]
+      >- (fs[endpoints_def,ALL_DISTINCT_APPEND] >>
+          metis_tac[trans_alt_par_l])
+      >- (metis_tac[trans_alt_par_l,trans_alt_par_r])
+      >- (metis_tac[trans_alt_par_l,trans_alt_par_r]))
+  >- (* Par-R *)
+     (qhdtm_x_assum `trans_alt` (assume_tac o SIMP_RULE std_ss [Once trans_alt_cases]) >>
+      fs[] >> rveq >> fs[] >> rveq >> fs[]
+      >- metis_tac[trans_alt_par_l,trans_alt_par_r] >>
+      fs[endpoints_def,ALL_DISTINCT_APPEND] >>
+      metis_tac[trans_alt_par_r,trans_alt_par_l])
+  >- (* trans_alt_fix *)
+     (qhdtm_x_assum `trans_alt` (assume_tac o SIMP_RULE std_ss [Once trans_alt_cases]) >>
+      fs[] >> rveq >> fs[] >> rveq >> fs[])
+  >- (* trans_alt_letrec *)
+     (qhdtm_x_assum `trans_alt` (assume_tac o SIMP_RULE std_ss [Once trans_alt_cases]) >>
+      fs[] >> rveq >> fs[] >> rveq >> fs[])
+  >- (* trans_alt_call *)
+     (qhdtm_x_assum `trans_alt` (assume_tac o SIMP_RULE std_ss [Once trans_alt_cases]) >>
+      fs[] >> rveq >> fs[] >> rveq >> fs[])
+QED
+
+Theorem payload_local_confluence_receive_alt:
+  ∀conf p1 s1 d1 r1 p2 p3 s2 d2 r2.
+  trans_alt conf p1 (LReceive s1 d1 r1) p2 /\ trans_alt conf p1 (LReceive s2 d2 r2) p3 /\ s1 <> s2
+  ==>
+  ?p4. trans_alt conf p2 (LReceive s2 d2 r2) p4 /\
+        trans_alt conf p3 (LReceive s1 d1 r1) p4
+Proof
+  `∀conf p1 alpha p2 s1 d1 r1 p3 s2 d2 r2.
+  trans_alt conf p1 alpha p2 /\ alpha = LReceive s1 d1 r1 /\
+  trans_alt conf p1 (LReceive s2 d2 r2) p3 /\ s1 <> s2
+  ==>
+  ?p4. trans_alt conf p2 (LReceive s2 d2 r2) p4 /\
+        trans_alt conf p3 (LReceive s1 d1 r1) p4` suffices_by metis_tac[] >>
+  Ho_Rewrite.PURE_REWRITE_TAC[GSYM AND_IMP_INTRO, GSYM PULL_FORALL]
+  >> ho_match_mp_tac trans_alt_strongind
+  >> rpt strip_tac >> fs[] >> rveq
+  >- (* Enqueue *)
+     (qhdtm_x_assum `trans_alt` (assume_tac o SIMP_RULE std_ss [Once trans_alt_cases]) >>
+      fs[] >> rveq >> fs[] >> rveq >> fs[] >>
+      qmatch_goalsub_abbrev_tac `NEndpoint p2 s1 e` >>
+      dxrule trans_alt_enqueue >> disch_then(qspecl_then [`conf`,`s1`,`d2`,`e`] mp_tac) >>
+      unabbrev_all_tac >> strip_tac >>
+      asm_exists_tac >> simp[] >>
+      qmatch_goalsub_abbrev_tac `NEndpoint p2 s1 e` >>
+      qpat_x_assum `_ <> _` mp_tac >>
+      dxrule trans_alt_enqueue >> disch_then(qspecl_then [`conf`,`s1`,`d`,`e`] mp_tac) >>
+      unabbrev_all_tac >> rpt strip_tac >>
+      simp[] >> fs[qpush_commute])
+  >- (* Par-L *)
+     (qhdtm_x_assum `trans_alt` (assume_tac o SIMP_RULE std_ss [Once trans_alt_cases]) >>
+      fs[] >> rveq >> fs[] >> rveq >> fs[] >>
+      metis_tac[trans_alt_par_l,trans_alt_par_r])
+  >- (* Par-R *)
+     (qhdtm_x_assum `trans_alt` (assume_tac o SIMP_RULE std_ss [Once trans_alt_cases]) >>
+      fs[] >> rveq >> fs[] >> rveq >> fs[] >>
+      metis_tac[trans_alt_par_l,trans_alt_par_r])
+QED
+
+Theorem trans_alt_let'':
+  ∀conf s v p f vl e q.
+         EVERY IS_SOME (MAP (FLOOKUP s.bindings) vl) ⇒
+         trans_alt conf (NEndpoint p (s with queues:= q) (Let v f vl e)) LTau
+           (NEndpoint p
+              (s with<|
+                 bindings := s.bindings |+ (v,f (MAP (THE ∘ FLOOKUP s.bindings) vl));
+                 queues:= q
+                 |>) e)
+Proof
+  rw[Once trans_alt_cases]
+QED
+
+Theorem trans_alt_dequeue_last_payload':
+  ∀conf s1 s2 v p1 p2 e d tl ds q.
+     p1 ≠ p2 ∧ qlk s1.queues p1 = d::tl ∧ final d ∧
+     s2.funs = s1.funs ∧
+     s2.bindings = s1.bindings |+ (v,FLAT (SNOC (unpad d) ds)) ∧
+     s2.queues = normalise_queues(s1.queues |+ (p1,tl))
+     ⇒
+     trans_alt conf (NEndpoint p2 s1 (Receive p1 v ds e)) LTau
+       (NEndpoint p2 s2 e)
+Proof
+  rw[Once trans_alt_cases] >> rw[state_component_equality]
+QED
+
+Theorem trans_alt_dequeue_intermediate_payload':
+  ∀conf s1 s2 v p1 p2 e d ds tl.
+     p1 ≠ p2 ∧ qlk s1.queues p1 = d::tl ∧ intermediate d ∧
+     s2.funs = s1.funs ∧
+     s2.bindings = s1.bindings ∧
+     s2.queues = normalise_queues(s1.queues |+ (p1,tl))
+      ⇒
+     trans_alt conf (NEndpoint p2 s1 (Receive p1 v ds e)) LTau
+       (NEndpoint p2 s2
+          (Receive p1 v (SNOC (unpad d) ds) e))
+Proof
+  rw[Once trans_alt_cases] >> rw[state_component_equality]
+QED
+
+Theorem trans_alt_same_receiver_determ:
+  trans_alt conf p1 (LReceive s d r) p2
+  /\ trans_alt conf p1 (LReceive s d r) p3
+  /\ ALL_DISTINCT(MAP FST(endpoints p1))
+  ==> p2 = p3
+Proof
+  metis_tac[trans_same_receiver_determ,trans_alt_nontau_eq,label_distinct]
+QED
+
+Theorem trans_alt_no_selfloop:
+  !conf p1 alpha p2.
+  trans_alt conf p1 alpha p2 ∧ conf.payload_size > 0 ∧ alpha ≠ LTau
+  ==> p1 <> p2
+Proof
+  metis_tac[trans_no_selfloop,trans_alt_nontau_eq,label_distinct]
+QED
+
+Theorem trans_alt_distinct_residual:
+  !conf p1 alpha p2 beta p3.
+  trans_alt conf p1 alpha p2
+  /\ trans_alt conf p1 beta p3
+  /\ alpha <> beta
+  /\ conf.payload_size > 0
+  ==> p2 <> p3
+Proof
+  Ho_Rewrite.PURE_REWRITE_TAC[GSYM PULL_FORALL,GSYM AND_IMP_INTRO] >>
+  ho_match_mp_tac trans_alt_strongind >> rpt strip_tac >>
+  fs[] >> rveq
+  >- (* Send-last-payload *)
+     (qhdtm_x_assum `trans_alt` (assume_tac o SIMP_RULE std_ss [Once trans_alt_cases]) >>
+      fs[] >> rveq >> fs[] >> rveq >> fs[payloadLangTheory.state_component_equality])
+  >- (* Send-intermediate-payload *)
+     (qhdtm_x_assum `trans_alt` (assume_tac o SIMP_RULE std_ss [Once trans_alt_cases]) >>
+      fs[] >> rveq >> fs[] >> rveq >> fs[payloadLangTheory.state_component_equality])
+  >- (* Enqueue *)
+     (qhdtm_x_assum `trans_alt` (assume_tac o SIMP_RULE std_ss [Once trans_alt_cases]) >>
+      fs[] >> rveq >> fs[] >> rveq >> fs[payloadLangTheory.state_component_equality] >>
+      qmatch_asmsub_abbrev_tac `a1:endpoint = a2` >>
+      `endpoint_size a1 = endpoint_size a2` by simp[] >>
+      unabbrev_all_tac >> pop_assum mp_tac >> rpt(pop_assum kall_tac) >>
+      simp[endpoint_size_def])
+  >- (* Com-L *)
+     (qhdtm_x_assum `trans_alt` (assume_tac o SIMP_RULE std_ss [Once trans_alt_cases]) >>
+      fs[] >> rveq >> fs[] >> rveq >> fs[] >>
+      Cases_on `beta` >> fs[] >> metis_tac[trans_alt_no_selfloop,label_distinct])
+  >- (* Com-R *)
+     (qhdtm_x_assum `trans_alt` (assume_tac o SIMP_RULE std_ss [Once trans_alt_cases]) >>
+      fs[] >> rveq >> fs[] >> rveq >> fs[] >>
+      Cases_on `beta` >> fs[] >> metis_tac[trans_alt_no_selfloop,label_distinct])
+  >- (* Dequeue-last-payload *)
+     (qhdtm_x_assum `trans_alt` (assume_tac o SIMP_RULE std_ss [Once trans_alt_cases]) >>
+      fs[] >> rveq >> fs[] >> rveq >> fs[payloadLangTheory.state_component_equality] >>
+      qmatch_asmsub_abbrev_tac `a1:endpoint = a2` >>
+      `endpoint_size a1 = endpoint_size a2` by simp[] >>
+      unabbrev_all_tac >> pop_assum mp_tac >> rpt(pop_assum kall_tac) >>
+      simp[endpoint_size_def])
+  >- (* Dequeue-intermediate-payload *)
+     (qhdtm_x_assum `trans_alt` (assume_tac o SIMP_RULE std_ss [Once trans_alt_cases]) >>
+      fs[] >> rveq >> fs[] >> rveq >> fs[payloadLangTheory.state_component_equality] >>
+      qmatch_asmsub_abbrev_tac `a1:endpoint = a2` >>
+      `endpoint_size a1 = endpoint_size a2` by simp[] >>
+      unabbrev_all_tac >> pop_assum mp_tac >> rpt(pop_assum kall_tac) >>
+      simp[endpoint_size_def])
+  >- (* If-L *)
+     (qhdtm_x_assum `trans_alt` (assume_tac o SIMP_RULE std_ss [Once trans_alt_cases]) >>
+      fs[] >> rveq >> fs[] >> rveq >> fs[payloadLangTheory.state_component_equality])
+  >- (* If-R *)
+     (qhdtm_x_assum `trans_alt` (assume_tac o SIMP_RULE std_ss [Once trans_alt_cases]) >>
+      fs[] >> rveq >> fs[] >> rveq >> fs[payloadLangTheory.state_component_equality])
+  >- (* Let *)
+     (qhdtm_x_assum `trans_alt` (assume_tac o SIMP_RULE std_ss [Once trans_alt_cases]) >>
+      fs[] >> rveq >> fs[] >> rveq >> fs[payloadLangTheory.state_component_equality])
+  >- (* Par-L *)
+     (qhdtm_x_assum `trans_alt` (assume_tac o SIMP_RULE std_ss [Once trans_alt_cases]) >>
+      fs[] >> rveq >> fs[] >> rveq >> fs[] >> metis_tac[trans_alt_no_selfloop,label_distinct])
+  >- (* Par-R *)
+     (qhdtm_x_assum `trans_alt` (assume_tac o SIMP_RULE std_ss [Once trans_alt_cases]) >>
+      fs[] >> rveq >> fs[] >> rveq >> fs[] >> metis_tac[trans_alt_no_selfloop,label_distinct])
+  >- (* Fix *)
+     (qhdtm_x_assum `trans_alt` (assume_tac o SIMP_RULE std_ss [Once trans_alt_cases]) >>
+      fs[] >> rveq >> fs[] >> rveq >> fs[state_component_equality])
+  >- (* Letrec *)
+     (qhdtm_x_assum `trans_alt` (assume_tac o SIMP_RULE std_ss [Once trans_alt_cases]) >>
+      fs[] >> rveq >> fs[] >> rveq >> fs[state_component_equality])
+  >- (* Call *)
+     (qhdtm_x_assum `trans_alt` (assume_tac o SIMP_RULE std_ss [Once trans_alt_cases]) >>
+      fs[] >> rveq >> fs[] >> rveq >> fs[state_component_equality])
+QED
+
+Theorem payload_local_confluence_tau_receive_alt:
+  ∀conf p1 p2 p3 s d r.
+  trans_alt conf p1 LTau p2 /\ trans_alt conf p1 (LReceive s d r) p3 /\ p2 <> p3 /\
+  ALL_DISTINCT (MAP FST (endpoints p1)) /\
+  ~MEM s (MAP FST (endpoints p1)) /\
+  conf.payload_size > 0
+  ==>
+  ?p4. trans_alt conf p2 (LReceive s d r) p4 /\
+        trans_alt conf p3 LTau p4
+Proof
+  `∀conf p1 alpha p2 p3 s d r.
+  trans_alt conf p1 alpha p2 /\ alpha = LTau /\ trans_alt conf p1 (LReceive s d r) p3 /\ p2 <> p3 /\
+  ALL_DISTINCT (MAP FST (endpoints p1)) /\
+  ~MEM s (MAP FST (endpoints p1)) /\
+  conf.payload_size > 0
+  ==>
+  ?p4. trans_alt conf p2 (LReceive s d r) p4 /\
+        trans_alt conf p3 LTau p4` suffices_by metis_tac[]
+  >> Ho_Rewrite.PURE_REWRITE_TAC[GSYM AND_IMP_INTRO, GSYM PULL_FORALL]
+  >> ho_match_mp_tac trans_alt_strongind
+  >> rpt strip_tac >> fs[] >> rveq
+  >- (* Com-L *)
+     (qhdtm_x_assum `trans_alt` (assume_tac o SIMP_RULE std_ss [Once trans_alt_cases]) >>
+      fs[] >> rveq >> fs[] >> rveq >> fs[]
+      >- (fs[endpoints_def,ALL_DISTINCT_APPEND] >>
+          drule payload_local_confluence_send_alt >> disch_then drule >>
+          impl_tac >-
+            (simp[] >> metis_tac[sender_is_endpoint_alt,receiver_is_endpoint_alt]) >>
+          strip_tac >>
+          metis_tac[trans_alt_com_l,trans_alt_par_l])
+      >- (fs[endpoints_def,ALL_DISTINCT_APPEND] >>
+          drule payload_local_confluence_send_alt >> disch_then drule >>
+          impl_tac >-
+            (simp[] >>
+             metis_tac[trans_alt_distinct_residual,sender_is_endpoint_alt,
+                       receiver_is_endpoint_alt,label_distinct]) >>
+          strip_tac >>
+          metis_tac[trans_alt_com_l,trans_alt_par_l]
+         )
+      >- (fs[endpoints_def,ALL_DISTINCT_APPEND] >>
+          imp_res_tac receiver_is_endpoint_alt >>
+          imp_res_tac sender_is_endpoint_alt >>
+          dxrule payload_local_confluence_receive_alt >>
+          disch_then dxrule >>
+          impl_tac >- metis_tac[] >>
+          strip_tac >>
+          metis_tac[trans_alt_com_l,trans_alt_par_r])
+      >- (fs[endpoints_def,ALL_DISTINCT_APPEND] >>
+          imp_res_tac receiver_is_endpoint_alt >>
+          imp_res_tac sender_is_endpoint_alt >>
+          dxrule payload_local_confluence_receive_alt >>
+          disch_then dxrule >>
+          impl_tac >- metis_tac[] >>
+          strip_tac >>
+          metis_tac[trans_alt_com_l,trans_alt_par_r]))
+  >- (* Com-R *)
+     (qhdtm_x_assum `trans_alt` (assume_tac o SIMP_RULE std_ss [Once trans_alt_cases]) >>
+      fs[] >> rveq >> fs[] >> rveq >> fs[]
+      >- (fs[endpoints_def,ALL_DISTINCT_APPEND] >>
+          imp_res_tac receiver_is_endpoint_alt >>
+          imp_res_tac sender_is_endpoint_alt >>
+          dxrule payload_local_confluence_receive_alt >>
+          disch_then dxrule >>
+          impl_tac >- metis_tac[] >>
+          strip_tac >>
+          metis_tac[trans_alt_com_r,trans_alt_par_l])
+      >- (fs[endpoints_def,ALL_DISTINCT_APPEND] >>
+          imp_res_tac receiver_is_endpoint_alt >>
+          imp_res_tac sender_is_endpoint_alt >>
+          dxrule payload_local_confluence_receive_alt >>
+          disch_then dxrule >>
+          impl_tac >- metis_tac[] >>
+          strip_tac >>
+          metis_tac[trans_alt_com_r,trans_alt_par_l])
+      >- (fs[endpoints_def,ALL_DISTINCT_APPEND] >>
+          drule payload_local_confluence_send_alt >> disch_then drule >>
+          impl_tac >-
+            (simp[] >>
+             metis_tac[sender_is_endpoint_alt,receiver_is_endpoint_alt,trans_alt_distinct_residual,
+                       label_distinct]) >>
+          strip_tac >>
+          metis_tac[trans_alt_com_r,trans_alt_par_r])
+      >- (fs[endpoints_def,ALL_DISTINCT_APPEND] >>
+          drule payload_local_confluence_send_alt >> disch_then drule >>
+          impl_tac >-
+            (simp[] >>
+             metis_tac[sender_is_endpoint_alt,receiver_is_endpoint_alt,trans_alt_distinct_residual,
+                       label_distinct]) >>
+          strip_tac >>
+          metis_tac[trans_alt_com_r,trans_alt_par_r]))
+  >- (* Dequeue-last-payload *)
+     (qhdtm_x_assum `trans_alt` (assume_tac o SIMP_RULE std_ss [Once trans_alt_cases]) >>
+      fs[] >> rveq >> fs[] >> rveq >> fs[] >>
+      qmatch_goalsub_abbrev_tac `trans_alt _ (NEndpoint p2 s1 e) (LReceive _ data _)` >>
+      dxrule trans_alt_enqueue >>
+      disch_then(qspecl_then [`conf`,`s1`,`data`,`e`] assume_tac) >>
+      asm_exists_tac >> simp[] >> unabbrev_all_tac >>
+      fs[endpoints_def] >>
+      rename1 ‘qpush _ p3 d2’ >>
+      (Cases_on ‘p1 = p3’ >-
+         (dep_rewrite.DEP_REWRITE_TAC[trans_alt_dequeue_last_payload'] >>
+          fs[qpush_def,qlk_def,fget_def,FLOOKUP_UPDATE,CaseEq"option",SNOC_APPEND,
+             normalise_queues_FUPDATE_NONEMPTY] >>
+          rw[fmap_eq_flookup,FLOOKUP_UPDATE] >> rw[DRESTRICT_normalise_queues,FLOOKUP_DRESTRICT]
+         ) >>
+       dep_rewrite.DEP_REWRITE_TAC[trans_alt_dequeue_last_payload'] >>
+       fs[qpush_def,qlk_def,fget_def,FLOOKUP_UPDATE,CaseEq"option",SNOC_APPEND] >>
+       fs[FUPDATE_COMMUTES] >>
+       rw[normalise_queues_FUPDATE_NONEMPTY]
+      ))
+  >- (* Dequeue-intermediate-payload *)
+     (qhdtm_x_assum `trans_alt` (assume_tac o SIMP_RULE std_ss [Once trans_alt_cases]) >>
+      fs[] >> rveq >> fs[] >> rveq >> fs[] >>
+      qmatch_goalsub_abbrev_tac `trans_alt _ (NEndpoint p2 s1 e1) (LReceive _ data _)` >>
+      dxrule trans_alt_enqueue >>
+      disch_then(qspecl_then [`conf`,`s1`,`data`,`e1`] assume_tac) >>
+      asm_exists_tac >> simp[] >> unabbrev_all_tac >>
+      rename1 ‘qpush _ p3 d2’ >>
+      (Cases_on ‘p1 = p3’ >-
+         (dep_rewrite.DEP_REWRITE_TAC[trans_alt_dequeue_intermediate_payload'] >>
+          fs[qpush_def,qlk_def,fget_def,FLOOKUP_UPDATE,CaseEq"option",SNOC_APPEND] >>
+          rw[fmap_eq_flookup,FLOOKUP_UPDATE] >> rw[DRESTRICT_normalise_queues,FLOOKUP_DRESTRICT] >>
+          fs[FLOOKUP_normalise_queues_FUPDATE] >> rw[]
+          ) >>
+       dep_rewrite.DEP_REWRITE_TAC[trans_alt_dequeue_intermediate_payload'] >>
+       fs[qpush_def,qlk_def,fget_def,FLOOKUP_UPDATE,CaseEq"option",SNOC_APPEND] >>
+       fs[FUPDATE_COMMUTES] >> rw[normalise_queues_FUPDATE_NONEMPTY] >>
+       rw[fmap_eq_flookup,FLOOKUP_UPDATE] >> rw[DRESTRICT_normalise_queues,FLOOKUP_DRESTRICT] >>
+       fs[FLOOKUP_normalise_queues] >> every_case_tac >> fs[])
+     )
+  >- (* If-L *)
+     (qhdtm_x_assum `trans_alt` (assume_tac o SIMP_RULE std_ss [Once trans_alt_cases]) >>
+      fs[] >> rveq >> fs[] >> rveq >> fs[] >>
+      qmatch_goalsub_abbrev_tac `trans_alt _ (NEndpoint p2 s1 e1) (LReceive _ data _)` >>
+      dxrule trans_alt_enqueue >>
+      disch_then(qspecl_then [`conf`,`s1`,`data`,`e1`] assume_tac) >>
+      asm_exists_tac >> simp[] >> unabbrev_all_tac >>
+      match_mp_tac trans_alt_if_true >>
+      simp[]
+     )
+  >- (* If-R *)
+     (qhdtm_x_assum `trans_alt` (assume_tac o SIMP_RULE std_ss [Once trans_alt_cases]) >>
+      fs[] >> rveq >> fs[] >> rveq >> fs[] >>
+      qmatch_goalsub_abbrev_tac `trans_alt _ (NEndpoint p2 s1 ee) (LReceive _ data _)` >>
+      dxrule trans_alt_enqueue >>
+      disch_then(qspecl_then [`conf`,`s1`,`data`,`ee`] assume_tac) >>
+      asm_exists_tac >> simp[] >> unabbrev_all_tac >>
+      match_mp_tac trans_alt_if_false >>
+      simp[]
+     )
+  >- (* Let *)
+     (qhdtm_x_assum `trans_alt` (assume_tac o SIMP_RULE std_ss [Once trans_alt_cases]) >>
+      fs[] >> rveq >> fs[] >> rveq >> fs[] >>
+      qmatch_goalsub_abbrev_tac `trans_alt _ (NEndpoint p2 s1 ee) (LReceive _ data _)` >>
+      dxrule trans_alt_enqueue >>
+      disch_then(qspecl_then [`conf`,`s1`,`data`,`ee`] assume_tac) >>
+      asm_exists_tac >> simp[] >> unabbrev_all_tac >>
+      simp[] >>
+      match_mp_tac trans_alt_let'' >> simp[]
+     )
+  >- (* Par-L *)
+     (qhdtm_x_assum `trans_alt` (assume_tac o SIMP_RULE std_ss [Once trans_alt_cases]) >>
+      fs[] >> rveq >> fs[] >> rveq >> fs[]
+      >- (fs[endpoints_def,ALL_DISTINCT_APPEND] >>
+          metis_tac[trans_alt_par_l])
+      >- (metis_tac[trans_alt_par_l,trans_alt_par_r])
+      >- (metis_tac[trans_alt_par_l,trans_alt_par_r]))
+  >- (* Par-R *)
+     (qhdtm_x_assum `trans_alt` (assume_tac o SIMP_RULE std_ss [Once trans_alt_cases]) >>
+      fs[] >> rveq >> fs[] >> rveq >> fs[]
+      >- metis_tac[trans_alt_par_l,trans_alt_par_r] >>
+      fs[endpoints_def,ALL_DISTINCT_APPEND] >>
+      metis_tac[trans_alt_par_r,trans_alt_par_l])
+  >- (* Fix *)
+     (qhdtm_x_assum `trans_alt` (assume_tac o SIMP_RULE std_ss [Once trans_alt_cases]) >>
+      fs[] >> rveq >> fs[] >> rveq >>
+      metis_tac[trans_alt_fix,trans_alt_enqueue])
+  >- (* Letrec *)
+     (qhdtm_x_assum `trans_alt` (assume_tac o SIMP_RULE std_ss [Once trans_alt_cases]) >>
+      fs[] >> rveq >> fs[] >> rveq >>
+      PURE_ONCE_REWRITE_TAC[trans_alt_cases] >>
+      fs[PULL_EXISTS])
+  >- (* Call *)
+     (qhdtm_x_assum `trans_alt` (assume_tac o SIMP_RULE std_ss [Once trans_alt_cases]) >>
+      fs[] >> rveq >> fs[] >> rveq >>
+      PURE_ONCE_REWRITE_TAC[trans_alt_cases] >>
+      fs[PULL_EXISTS])
+QED
+
+Theorem payload_local_confluence_tau_alt:
+  ∀conf p1 p2 p3.
+  trans_alt conf p1 LTau p2 /\ trans_alt conf p1 LTau p3 /\ p2 <> p3 /\
+  ALL_DISTINCT (MAP FST (endpoints p1)) /\
+  conf.payload_size > 0
+  ==>
+  ?p4. trans_alt conf p2 LTau p4 /\
+        trans_alt conf p3 LTau p4
+Proof
+  `∀conf p1 alpha p2.
+    trans_alt conf p1 alpha p2 ==> !p3. alpha = LTau /\ trans_alt conf p1 LTau p3 /\ p2 <> p3 /\
+    ALL_DISTINCT (MAP FST (endpoints p1)) /\ conf.payload_size > 0
+    ==>
+    ?p4. trans_alt conf p2 LTau p4 /\
+            trans_alt conf p3 LTau p4` suffices_by metis_tac[]
+  >> ho_match_mp_tac trans_alt_strongind
+  >> rpt strip_tac >> fs[] >> rveq
+  >- (* Com-L *)
+     (qhdtm_x_assum `trans_alt` (assume_tac o SIMP_RULE std_ss [Once trans_alt_cases]) >>
+      fs[] >> rveq >> fs[] >> rveq >> fs[endpoints_def,ALL_DISTINCT_APPEND]
+      >- (qmatch_asmsub_abbrev_tac `trans_alt _ _ (LSend s1 _ _)` >>
+          qpat_x_assum `trans_alt _ _ (LSend _ _ _) _` mp_tac >>
+          qmatch_asmsub_abbrev_tac `trans_alt _ _ (LSend s2 _ _)` >>
+          strip_tac >>
+          rpt(qhdtm_x_assum `Abbrev` kall_tac) >>
+          Cases_on `s1 = s2` >-
+            (rveq >>
+             fs[endpoints_def,ALL_DISTINCT_APPEND] >>
+             dxrule_all_then strip_assume_tac trans_alt_same_sender_determ >>
+             rveq >> fs[]) >>
+          imp_res_tac sender_is_endpoint_alt >>
+          imp_res_tac receiver_is_endpoint_alt >>
+          dxrule payload_local_confluence_send_alt >>
+          disch_then dxrule >>
+          impl_tac >- (simp[] >> metis_tac[]) >>
+          strip_tac >>
+          dxrule_all_then strip_assume_tac payload_local_confluence_receive_alt >>
+          metis_tac[trans_alt_com_l])
+      >- (qmatch_asmsub_abbrev_tac `trans_alt _ _ (LSend s1 _ _)` >>
+          qpat_x_assum `trans_alt _ _ (LSend _ _ _) _` mp_tac >>
+          qmatch_asmsub_abbrev_tac `trans_alt _ _ (LSend s2 _ _)` >>
+          strip_tac >>
+          rpt(qhdtm_x_assum `Abbrev` kall_tac) >>
+          Cases_on `s1 = s2` >-
+            (rveq >>
+             fs[endpoints_def,ALL_DISTINCT_APPEND] >>
+             dxrule_all_then strip_assume_tac trans_alt_same_sender_determ >>
+             rveq >> fs[] >> metis_tac[trans_alt_same_receiver_determ]) >>
+          imp_res_tac sender_is_endpoint_alt >>
+          imp_res_tac receiver_is_endpoint_alt >>
+          drule_then assume_tac (GEN_ALL trans_alt_different_sender) >>
+          qpat_x_assum `trans_alt _ _ (LSend _ _ _) _` mp_tac >>
+          first_x_assum drule >> impl_tac >- simp[] >>
+          rpt strip_tac >>
+          dxrule payload_local_confluence_send_alt >>
+          disch_then dxrule >>
+          impl_tac >- (simp[] >> metis_tac[]) >>
+          strip_tac >>
+          dxrule_all_then strip_assume_tac payload_local_confluence_receive_alt >>
+          metis_tac[trans_alt_com_l])
+      >- (imp_res_tac sender_is_endpoint_alt >>
+          imp_res_tac receiver_is_endpoint_alt >>
+          drule(GEN_ALL trans_alt_send_receive_distinct) >>
+          disch_then drule >> impl_tac >- simp[] >>
+          strip_tac >>
+          qpat_x_assum `trans_alt _ _ (LSend _ _ _) _` mp_tac >>
+          dxrule_then assume_tac payload_local_confluence_send_alt >>
+          strip_tac >> first_x_assum dxrule >>
+          impl_tac >- (simp[] >> metis_tac[]) >>
+          qpat_x_assum `trans_alt _ _ (LSend _ _ _) _` mp_tac >>
+          dxrule_then assume_tac payload_local_confluence_send_alt >>
+          strip_tac >> first_x_assum dxrule >>
+          impl_tac >- simp[] >>
+          rpt strip_tac >>
+          metis_tac[trans_alt_com_l,trans_alt_com_r])
+      >- (imp_res_tac sender_is_endpoint_alt >>
+          imp_res_tac receiver_is_endpoint_alt >>
+          qpat_x_assum `trans_alt _ _ (LSend _ _ _) _` mp_tac >>
+          drule(GEN_ALL trans_alt_send_receive_distinct) >>
+          disch_then drule >> impl_tac >- simp[] >>
+          strip_tac >>
+          dxrule_then assume_tac payload_local_confluence_send_alt >>
+          strip_tac >> first_x_assum dxrule >>
+          impl_tac >- (simp[] >> metis_tac[]) >>
+          qpat_x_assum `trans_alt _ _ (LSend _ _ _) _` mp_tac >>
+          dxrule_then assume_tac payload_local_confluence_send_alt >>
+          strip_tac >> first_x_assum dxrule >>
+          impl_tac >- simp[] >>
+          rpt strip_tac >>
+          metis_tac[trans_alt_com_l,trans_alt_com_r])
+      >- (imp_res_tac sender_is_endpoint_alt >>
+          imp_res_tac receiver_is_endpoint_alt >>
+          dxrule payload_local_confluence_send_alt >>
+          disch_then dxrule >>
+          impl_tac >- (simp[] >> metis_tac[]) >>
+          strip_tac >>
+          metis_tac[trans_alt_com_l,trans_alt_par_l])
+      >- (imp_res_tac sender_is_endpoint_alt >>
+          imp_res_tac receiver_is_endpoint_alt >>
+          drule_then assume_tac trans_alt_distinct_residual >>
+          qhdtm_x_assum `trans_alt` mp_tac >>
+          pop_assum drule >> impl_tac >- simp[] >>
+          rpt strip_tac >>
+          dxrule payload_local_confluence_send_alt >>
+          disch_then dxrule >>
+          impl_tac >- (simp[] >> metis_tac[]) >>
+          strip_tac >>
+          metis_tac[trans_alt_com_l,trans_alt_par_l])
+      >- (imp_res_tac sender_is_endpoint_alt >>
+          imp_res_tac receiver_is_endpoint_alt >>
+          drule_then assume_tac trans_alt_distinct_residual >>
+          qhdtm_x_assum `trans_alt` mp_tac >>
+          pop_assum drule >> impl_tac >- simp[] >>
+          rpt strip_tac >>
+          dxrule payload_local_confluence_tau_receive_alt >>
+          disch_then dxrule >>
+          impl_tac >- (simp[] >> metis_tac[]) >>
+          strip_tac >>
+          metis_tac[trans_alt_com_l,trans_alt_par_r])
+      >- (imp_res_tac sender_is_endpoint_alt >>
+          imp_res_tac receiver_is_endpoint_alt >>
+          drule_then assume_tac trans_alt_distinct_residual >>
+          qhdtm_x_assum `trans_alt` mp_tac >>
+          pop_assum drule >> impl_tac >- simp[] >>
+          rpt strip_tac >>
+          dxrule payload_local_confluence_tau_receive_alt >>
+          disch_then dxrule >>
+          impl_tac >- (simp[] >> metis_tac[]) >>
+          strip_tac >>
+          metis_tac[trans_alt_com_l,trans_alt_par_r]))
+  >- (* Com-R *)
+     (qhdtm_x_assum `trans_alt` (assume_tac o SIMP_RULE std_ss [Once trans_alt_cases]) >>
+      fs[] >> rveq >> fs[] >> rveq >> fs[endpoints_def,ALL_DISTINCT_APPEND]
+      >- (imp_res_tac sender_is_endpoint_alt >>
+          imp_res_tac receiver_is_endpoint_alt >>
+          qpat_x_assum `trans_alt _ _ (LSend _ _ _) _` mp_tac >>
+          drule(GEN_ALL trans_alt_send_receive_distinct) >>
+          disch_then drule >> impl_tac >- simp[] >>
+          strip_tac >>
+          dxrule_then assume_tac payload_local_confluence_send_alt >>
+          strip_tac >> first_x_assum dxrule >>
+          impl_tac >- (simp[] >> metis_tac[]) >>
+          qpat_x_assum `trans_alt _ _ (LSend _ _ _) _` mp_tac >>
+          dxrule_then assume_tac payload_local_confluence_send_alt >>
+          strip_tac >> first_x_assum dxrule >>
+          impl_tac >- (simp[] >> metis_tac[]) >>
+          rpt strip_tac >>
+          metis_tac[trans_alt_com_l,trans_alt_com_r])
+      >- (imp_res_tac sender_is_endpoint_alt >>
+          imp_res_tac receiver_is_endpoint_alt >>
+          drule(GEN_ALL trans_alt_send_receive_distinct) >>
+          disch_then drule >> impl_tac >- simp[] >>
+          strip_tac >>
+          qpat_x_assum `trans_alt _ _ (LSend _ _ _) _` mp_tac >>
+          dxrule_then assume_tac payload_local_confluence_send_alt >>
+          strip_tac >> first_x_assum dxrule >>
+          impl_tac >- (simp[] >> metis_tac[]) >>
+          qpat_x_assum `trans_alt _ _ (LSend _ _ _) _` mp_tac >>
+          dxrule_then assume_tac payload_local_confluence_send_alt >>
+          strip_tac >> first_x_assum dxrule >>
+          impl_tac >- (simp[] >> metis_tac[]) >>
+          rpt strip_tac >>
+          metis_tac[trans_alt_com_l,trans_alt_com_r])
+      >- (qmatch_asmsub_abbrev_tac `trans_alt _ _ (LSend s1 _ _)` >>
+          qpat_x_assum `trans_alt _ _ (LSend _ _ _) _` mp_tac >>
+          qmatch_asmsub_abbrev_tac `trans_alt _ _ (LSend s2 _ _)` >>
+          strip_tac >>
+          rpt(qhdtm_x_assum `Abbrev` kall_tac) >>
+          Cases_on `s1 = s2` >-
+            (rveq >>
+             fs[endpoints_def,ALL_DISTINCT_APPEND] >>
+             dxrule_all_then strip_assume_tac trans_alt_same_sender_determ >>
+             rveq >> fs[] >>
+             dxrule_all trans_alt_same_receiver_determ >> simp[]
+            ) >>
+          drule_then assume_tac (GEN_ALL trans_alt_different_sender) >>
+          pop_assum(qspec_then `s2` mp_tac) >>
+          disch_then drule >> impl_tac >- simp[] >>
+          strip_tac >>
+          imp_res_tac sender_is_endpoint_alt >>
+          imp_res_tac receiver_is_endpoint_alt >>
+          dxrule payload_local_confluence_send_alt >>
+          disch_then dxrule >>
+          impl_tac >- (simp[] >> metis_tac[]) >>
+          strip_tac >>
+          dxrule_all_then strip_assume_tac payload_local_confluence_receive_alt >>
+          metis_tac[trans_alt_com_r])
+      >- (qmatch_asmsub_abbrev_tac `trans_alt _ _ (LSend s1 _ _)` >>
+          qpat_x_assum `trans_alt _ _ (LSend _ _ _) _` mp_tac >>
+          qmatch_asmsub_abbrev_tac `trans_alt _ _ (LSend s2 _ _)` >>
+          strip_tac >>
+          rpt(qhdtm_x_assum `Abbrev` kall_tac) >>
+          Cases_on `s1 = s2` >-
+            (rveq >>
+             fs[endpoints_def,ALL_DISTINCT_APPEND] >>
+             dxrule_all_then strip_assume_tac trans_alt_same_sender_determ >>
+             rveq >> fs[] >>
+             dxrule_all trans_alt_same_receiver_determ >> simp[]
+            ) >>
+          drule_then assume_tac (GEN_ALL trans_alt_different_sender) >>
+          pop_assum(qspec_then `s2` mp_tac) >>
+          disch_then drule >> impl_tac >- simp[] >>
+          strip_tac >>
+          imp_res_tac sender_is_endpoint_alt >>
+          imp_res_tac receiver_is_endpoint_alt >>
+          dxrule payload_local_confluence_send_alt >>
+          disch_then dxrule >>
+          impl_tac >- (simp[] >> metis_tac[]) >>
+          strip_tac >>
+          dxrule_all_then strip_assume_tac payload_local_confluence_receive_alt >>
+          metis_tac[trans_alt_com_r])
+      >- (imp_res_tac sender_is_endpoint_alt >>
+          imp_res_tac receiver_is_endpoint_alt >>
+          dxrule payload_local_confluence_tau_receive_alt >>
+          disch_then dxrule >>
+          impl_tac >- (simp[] >> metis_tac[]) >>
+          strip_tac >>
+          metis_tac[trans_alt_com_r,trans_alt_par_l]
+         )
+      >- (imp_res_tac sender_is_endpoint_alt >>
+          imp_res_tac receiver_is_endpoint_alt >>
+          drule_then assume_tac trans_alt_distinct_residual >>
+          qhdtm_x_assum `trans_alt` mp_tac >>
+          pop_assum drule >> impl_tac >- simp[] >>
+          rpt strip_tac >>
+          dxrule payload_local_confluence_tau_receive_alt >>
+          disch_then dxrule >>
+          impl_tac >- (simp[] >> metis_tac[]) >>
+          strip_tac >>
+          metis_tac[trans_alt_com_r,trans_alt_par_l])
+      >- (imp_res_tac sender_is_endpoint_alt >>
+          imp_res_tac receiver_is_endpoint_alt >>
+          drule_then assume_tac trans_alt_distinct_residual >>
+          qhdtm_x_assum `trans_alt` mp_tac >>
+          pop_assum drule >> impl_tac >- simp[] >>
+          rpt strip_tac >>
+          dxrule payload_local_confluence_send_alt >>
+          disch_then dxrule >>
+          impl_tac >- (simp[] >> metis_tac[]) >>
+          strip_tac >>
+          metis_tac[trans_alt_com_r,trans_alt_par_r])
+      >- (imp_res_tac sender_is_endpoint_alt >>
+          imp_res_tac receiver_is_endpoint_alt >>
+          drule_then assume_tac trans_alt_distinct_residual >>
+          qhdtm_x_assum `trans_alt` mp_tac >>
+          pop_assum drule >> impl_tac >- simp[] >>
+          rpt strip_tac >>
+          dxrule payload_local_confluence_send_alt >>
+          disch_then dxrule >>
+          impl_tac >- (simp[] >> metis_tac[]) >>
+          strip_tac >>
+          metis_tac[trans_alt_com_r,trans_alt_par_r]))
+  >- (* Dequeue-last-payload *)
+     (qhdtm_x_assum `trans_alt` (assume_tac o SIMP_RULE std_ss [Once trans_alt_cases]) >>
+      fs[] >> rveq >> fs[] >> rveq >> fs[] >>
+      fs[APPEND_EQ_APPEND_MID] >> rveq >>
+      fs[APPEND_EQ_SING |> CONV_RULE(LHS_CONV SYM_CONV)] >>
+      rveq >> fs[] >>
+      imp_res_tac intermediate_final_IMP)
+  >- (* Dequeue-intermediate-payload *)
+     (qhdtm_x_assum `trans_alt` (assume_tac o SIMP_RULE std_ss [Once trans_alt_cases]) >>
+      fs[] >> rveq >> fs[] >> rveq >> fs[] >>
+      fs[APPEND_EQ_APPEND_MID] >> rveq >>
+      fs[APPEND_EQ_SING |> CONV_RULE(LHS_CONV SYM_CONV)] >>
+      rveq >> fs[] >>
+      imp_res_tac intermediate_final_IMP)
+  >- (* If-L *)
+     (qhdtm_x_assum `trans_alt` (assume_tac o SIMP_RULE std_ss [Once trans_alt_cases]) >>
+      fs[] >> rveq >> fs[])
+  >- (* If-R *)
+     (qhdtm_x_assum `trans_alt` (assume_tac o SIMP_RULE std_ss [Once trans_alt_cases]) >>
+      fs[] >> rveq >> fs[])
+  >- (* Let *)
+     (qhdtm_x_assum `trans_alt` (assume_tac o SIMP_RULE std_ss [Once trans_alt_cases]) >>
+      fs[] >> rveq >> fs[])
+  >- (* Par-L *)
+     (qhdtm_x_assum `trans_alt` (assume_tac o SIMP_RULE std_ss [Once trans_alt_cases]) >>
+      fs[] >> rveq >> fs[] >> rveq >> fs[]
+      >- (fs[endpoints_def,ALL_DISTINCT_APPEND] >>
+          qpat_x_assum `_ _ _ LTau _` assume_tac >>
+          drule payload_local_confluence_send_alt >>
+          disch_then drule >>
+          impl_tac >- metis_tac[receiver_is_endpoint_alt] >>
+          strip_tac >>
+          metis_tac[trans_alt_com_l,trans_alt_par_l])
+      >- (fs[endpoints_def,ALL_DISTINCT_APPEND] >>
+          qpat_x_assum `_ _ _ LTau _` assume_tac >>
+          drule payload_local_confluence_send_alt >>
+          disch_then drule >>
+          impl_tac >- (simp[] >> metis_tac[trans_alt_distinct_residual,label_distinct,
+                                           sender_is_endpoint_alt,receiver_is_endpoint_alt]) >>
+          strip_tac >>
+          metis_tac[trans_alt_com_l,trans_alt_par_l])
+      >- (fs[endpoints_def,ALL_DISTINCT_APPEND] >>
+          imp_res_tac sender_is_endpoint_alt >>
+          imp_res_tac receiver_is_endpoint_alt >>
+          drule payload_local_confluence_tau_receive_alt >>
+          disch_then drule >>
+          impl_tac >- (simp[] >> metis_tac[]) >>
+          strip_tac >>
+          metis_tac[trans_alt_com_r,trans_alt_par_l])
+      >- (fs[endpoints_def,ALL_DISTINCT_APPEND] >>
+          imp_res_tac sender_is_endpoint_alt >>
+          imp_res_tac receiver_is_endpoint_alt >>
+          drule payload_local_confluence_tau_receive_alt >>
+          disch_then drule >>
+          impl_tac >- (simp[] >> metis_tac[trans_alt_distinct_residual,label_distinct]) >>
+          strip_tac >>
+          metis_tac[trans_alt_com_r,trans_alt_par_l])
+      >- (fs[endpoints_def,ALL_DISTINCT_APPEND] >>
+          metis_tac[trans_alt_par_l])
+      >- (fs[endpoints_def,ALL_DISTINCT_APPEND] >>
+          metis_tac[trans_alt_par_r,trans_alt_par_l])
+      >- (fs[endpoints_def,ALL_DISTINCT_APPEND] >>
+          metis_tac[trans_alt_par_r,trans_alt_par_l]))
+  >- (* Par-R *)
+     (qhdtm_x_assum `trans_alt` (assume_tac o SIMP_RULE std_ss [Once trans_alt_cases]) >>
+      fs[] >> rveq >> fs[] >> rveq >> fs[]
+      >- (fs[endpoints_def,ALL_DISTINCT_APPEND] >>
+          imp_res_tac sender_is_endpoint_alt >>
+          imp_res_tac receiver_is_endpoint_alt >>
+          drule payload_local_confluence_tau_receive_alt >>
+          disch_then drule >>
+          impl_tac >- (simp[] >> metis_tac[trans_alt_distinct_residual,label_distinct]) >>
+          strip_tac >>
+          metis_tac[trans_alt_com_l,trans_alt_par_r])
+      >- (fs[endpoints_def,ALL_DISTINCT_APPEND] >>
+          imp_res_tac sender_is_endpoint_alt >>
+          imp_res_tac receiver_is_endpoint_alt >>
+          drule payload_local_confluence_tau_receive_alt >>
+          disch_then drule >>
+          impl_tac >- (simp[] >> metis_tac[trans_alt_distinct_residual,label_distinct]) >>
+          strip_tac >>
+          metis_tac[trans_alt_com_l,trans_alt_par_r])
+      >- (fs[endpoints_def,ALL_DISTINCT_APPEND] >>
+          qpat_x_assum `_ _ _ LTau _` assume_tac >>
+          drule payload_local_confluence_send_alt >>
+          disch_then drule >>
+          impl_tac >- (simp[] >> metis_tac[trans_alt_distinct_residual,label_distinct,
+                                           sender_is_endpoint_alt,receiver_is_endpoint_alt]) >>
+          strip_tac >>
+          metis_tac[trans_alt_com_r,trans_alt_par_r])
+      >- (fs[endpoints_def,ALL_DISTINCT_APPEND] >>
+          qpat_x_assum `_ _ _ LTau _` assume_tac >>
+          drule payload_local_confluence_send_alt >>
+          disch_then drule >>
+          impl_tac >- (simp[] >> metis_tac[trans_alt_distinct_residual,label_distinct,
+                                           sender_is_endpoint_alt,receiver_is_endpoint_alt]) >>
+          strip_tac >>
+          metis_tac[trans_alt_com_r,trans_alt_par_r])
+      >- (dxrule_then (qspec_then `p2` assume_tac) trans_alt_par_l >>
+          asm_exists_tac >> simp[] >> pop_assum kall_tac >>
+          rename1 `NPar q` >>
+          dxrule_then (qspec_then `q` assume_tac) trans_alt_par_r >>
+          asm_exists_tac >> simp[])
+      >- (dxrule_then (qspec_then `p2` assume_tac) trans_alt_par_l >>
+          asm_exists_tac >> simp[] >> pop_assum kall_tac >>
+          rename1 `NPar q` >>
+          dxrule_then (qspec_then `q` assume_tac) trans_alt_par_r >>
+          asm_exists_tac >> simp[])
+      >- (fs[endpoints_def,ALL_DISTINCT_APPEND] >>
+          first_x_assum(drule_all_then strip_assume_tac) >>
+          imp_res_tac trans_alt_par_r >>
+          rpt(first_x_assum(qspec_then `n1` assume_tac)) >>
+          ntac 2 (asm_exists_tac >> simp[]) >>
+          metis_tac[]))
+  >- (* Fix *)
+     (qhdtm_x_assum `trans_alt` (assume_tac o SIMP_RULE std_ss [Once trans_alt_cases]) >>
+      fs[] >> rveq >> fs[] >> rveq >>
+      PURE_ONCE_REWRITE_TAC[trans_alt_cases] >>
+      fs[PULL_EXISTS])
+  >- (* Letrec *)
+     (qhdtm_x_assum `trans_alt` (assume_tac o SIMP_RULE std_ss [Once trans_alt_cases]) >>
+      fs[] >> rveq >> fs[] >> rveq >>
+      PURE_ONCE_REWRITE_TAC[trans_alt_cases] >>
+      fs[PULL_EXISTS])
+  >- (* Call *)
+     (qhdtm_x_assum `trans_alt` (assume_tac o SIMP_RULE std_ss [Once trans_alt_cases]) >>
+      fs[] >> rveq >> fs[] >> rveq >>
+      PURE_ONCE_REWRITE_TAC[trans_alt_cases] >>
+      fs[PULL_EXISTS])
+QED
+
+val list_trans_alt_def = Define `
+    (list_trans_alt conf p [] q = (p = q))
+ /\ (list_trans_alt conf p (alpha::l) q = ?p'. trans_alt conf p alpha p' /\ list_trans_alt conf p' l q)`
+
+val list_trans_alt_append = Q.store_thm("list_trans_alt_append",
+  `!l1 n1 l2 n2 conf. list_trans_alt conf n1 (l1 ++ l2) n2 =
+  ?n3. list_trans_alt conf n1 l1 n3 /\ list_trans_alt conf n3 l2 n2`,
+  Induct_on `l1` >> rpt strip_tac >> fs[list_trans_alt_def]
+  >> rw[EQ_IMP_THM] >> fs[] >> metis_tac[]);
+
+val endpoint_names_trans_alt = Q.store_thm("endpoint_names_trans_alt",
+  `!conf n1 alpha n2. trans_alt conf n1 alpha n2 ==> MAP FST (endpoints n2) = MAP FST(endpoints n1)`,
+  ho_match_mp_tac trans_alt_strongind >> rpt strip_tac >> fs[endpoints_def]);
+
+val endpoint_names_list_trans_alt = Q.store_thm("endpoint_names_list_trans_alt",
+  `!conf n1 alpha n2. list_trans_alt conf n1 alpha n2 ==> MAP FST (endpoints n2) = MAP FST(endpoints n1)`,
+  Induct_on `alpha` >> rw[list_trans_alt_def] >>
+  metis_tac[endpoint_names_trans_alt]);
+
+Theorem payload_confluence_contract_alt:
+  ∀m conf p1 p2 p3.
+   trans_alt conf p1 LTau p2 /\
+   list_trans_alt conf p1 (REPLICATE m LTau) p3 /\
+   ALL_DISTINCT (MAP FST (endpoints p1)) /\
+   conf.payload_size > 0
+   ==>
+   (?n. list_trans_alt conf p2 (REPLICATE n LTau) p3 /\
+        n <= m) \/
+   (?n p4. list_trans_alt conf p2 (REPLICATE n LTau) p4 /\
+        trans_alt conf p3 LTau p4 /\
+        n <= m)
+Proof
+  Induct >> rpt strip_tac
+  >- (fs[list_trans_alt_def] >> rveq >>
+      disj2_tac >> asm_exists_tac >> simp[])
+  >> FULL_SIMP_TAC bool_ss [REPLICATE_SUC_SNOC]
+  >> fs[list_trans_alt_append,list_trans_alt_def]
+  >> first_x_assum drule_all
+  >> strip_tac
+  >- (disj1_tac >>
+      qexists_tac ‘SUC n’ >>
+      PURE_REWRITE_TAC[REPLICATE_SUC_SNOC] >>
+      rw[list_trans_alt_append,list_trans_alt_def] >>
+      metis_tac[])
+  >- (Cases_on `p3 = p4`
+      >- (rveq >>
+          disj1_tac >> asm_exists_tac >>
+          simp[]) >>
+      disj2_tac >>
+      imp_res_tac endpoint_names_trans_alt >>
+      imp_res_tac endpoint_names_list_trans_alt >>
+      dxrule payload_local_confluence_tau_alt >>
+      disch_then dxrule >>
+      impl_tac >- simp[] >>
+      strip_tac >>
+      qexists_tac ‘SUC n’ >>
+      PURE_REWRITE_TAC[REPLICATE_SUC_SNOC] >>
+      rw[list_trans_alt_append,list_trans_alt_def] >>
+      metis_tac[])
+QED
+
+Theorem payload_confluence_weak_contract_alt:
+  ∀n m conf p1 p2 p3.
+   list_trans_alt conf p1 (REPLICATE n LTau) p2 /\
+   list_trans_alt conf p1 (REPLICATE m LTau) p3 /\
+   ALL_DISTINCT (MAP FST (endpoints p1)) /\
+   conf.payload_size > 0
+   ==>
+   (?n' m' p4. list_trans_alt conf p2 (REPLICATE n' LTau) p4 /\
+        list_trans_alt conf p3 (REPLICATE m' LTau) p4 /\
+        n' <= m /\ m' <= n)
+Proof
+  Induct >> rpt strip_tac
+  >- (fs[list_trans_alt_def] >> rveq >>
+      asm_exists_tac >> simp[])
+  >> FULL_SIMP_TAC bool_ss [REPLICATE_SUC_SNOC]
+  >> fs[list_trans_alt_append,list_trans_alt_def]
+  >> first_x_assum drule_all
+  >> strip_tac
+  >> drule payload_confluence_contract_alt
+  >> disch_then drule
+  >> impl_tac
+  >- (imp_res_tac endpoint_names_trans_alt >>
+      imp_res_tac endpoint_names_list_trans_alt >>
+      fs[])
+  >> strip_tac
+  >- (asm_exists_tac >> simp[] >> asm_exists_tac >> simp[] >> metis_tac[])
+  >> goal_assum drule >> simp[]
+  >> qexists_tac ‘SUC m'’
+  >> PURE_REWRITE_TAC[REPLICATE_SUC_SNOC]
+  >> rw[list_trans_alt_append,list_trans_alt_def]
+  >> metis_tac[]
 QED
 
 val _ = export_theory();
